\subsection{Таблица производных}
Здесь производная берётся по~переменной~$x$.
\begin{itemize}
	\item $(C)' = 0$
	
	\item $(x^n)' = nx^{n-1}, \ n \neq 0$
	\begin{proof}
	Пусть $h = x - a$.
	Пользуясь \hyperref[eq:binomial_expansion]{формулой бинома Ньютона}, получим
	\begin{equation*}
	(a^n)' =
	\lim_{h \to 0} \frac{(a + h)^n - a^n}h =
	\lim_{h \to 0} \frac{a^n - a^n + n a^{n-1} h + \frac12 n(n - 1) a^{n-2} h^2 + \ldots}h =
	\end{equation*}
	\begin{equation*}
	= n a^{n-1} + \lim_{h \to 0} \left( \frac12 n(n - 1) a^{n-2} h + \ldots \right) =
	n a^{n-1}
	\end{equation*}
	\end{proof}
	
	\item $(f^n(x))' = nf'(x)f^{n-1}(x), \ n \neq 0$
	
	\item $(|x|)' = \sgn x$
		
	\item $(\ln x)' = \dfrac1x$
	
	\item $(a^x)' = a^x \cdot \ln a, \ a > 0$
	
	\item $(a^{f(x)})' = a^x \cdot \ln a \cdot f'(x), \ a > 0$
	
	\item $(\sin x)' = \cos x$
	\begin{proof}
	\begin{equation*}
	\sin a =
	\lim_{x \to a} \frac{\sin x - \sin a}{x - a} =
	\lim_{x \to a} \frac{2 \cos \frac{x + a}2 \sin \frac{x - a}2}{x - a} =
	\lim_{x \to a} \frac{2 \sin \frac{x - a}2}{x - a} \cdot \lim_{x \to a} \cos \frac{x + a}2 =
	\cos a
	\end{equation*}
	\end{proof}
	
	\item $(\cos x)' = -\sin x$
	\begin{proof}
	\begin{equation*}
	(\cos x)' =
	(\sin \left( \frac\pi{2} - x \right))' =
	-\cos \left( \frac\pi{2} - x \right) =
	-\sin x
	\end{equation*}
	\end{proof}
	
	\item $(\tg x)' = \dfrac1{\cos^2 x}$
	\begin{proof}
	\begin{equation*}
	(\tg x)' =
	\left( \frac{\sin x}{\cos x} \right)' =
	\frac{\cos^2 x + \sin^2 x}{\cos^2 x} =
	\frac1{\cos^2 x}
	\end{equation*}
	\end{proof}
	
	\item $(\ctg x)' = -\dfrac1{\sin^2 x}$
	\begin{proof}
	\begin{equation*}
	(\ctg x)' =
	\left( \frac{\cos x}{\sin x} \right)' =
	\frac{-\sin^2 x - \cos^2 x}{\sin^2 x} =
	-\frac1{\sin^2 x}
	\end{equation*}
	\end{proof}
	
	\item $(\arcsin x)' = \dfrac1{\sqrt{1 - x^2}}$
	\begin{proof}
	\begin{equation*}
	(\arcsin x)' =
	\frac1{\cos \arcsin x} =
	\frac1{\sqrt{1 - \sin^2 \arcsin x}} =
	\frac1{\sqrt{1 - x^2}}
	\end{equation*}
	\end{proof}
	
	\item $(\arccos x)' = -\dfrac1{\sqrt{1 - x^2}}$
	\begin{proof}
	\begin{equation*}
	(\arccos x)' =
	\left( \frac\pi{2} - \arcsin x \right)' =
	-\frac1{\sqrt{1 - x^2}}
	\end{equation*}
	\end{proof}
	
	\item $(\arctg x)' = \dfrac1{1 + x^2}$
	\begin{proof}
	\begin{equation*}
	(\arctg x)' =
	\cos^2 \arctg x =
	\frac1{1 + \tg^2 \arctg x} =
	\frac1{1 + x^2}
	\end{equation*}
	\end{proof}
	
	\item $(\arcctg x)' = -\dfrac1{1 + x^2}$
	\begin{proof}
	\begin{equation*}
	(\arcctg x)' =
	\left( \frac\pi{2} - \arctg x \right)' =
	-\frac1{1 + x^2}
	\end{equation*}
	\end{proof}
\end{itemize}