\section{Алгебраические преобразования}
Формулы сокращённого умножения:
\begin{enumerate}
	\item Квадрат суммы:
	\begin{equation*}
	(a \pm b)^2 = (a \pm b)(a \pm b) = a^2 \pm 2ab + b^2
	\end{equation*}
	
	\item Разность квадратов:
	\begin{equation*}
	a^2 - b^2 = a^2 - ab + (ab - b^2) = (a + b)(a - b)
	\end{equation*}
	
	\item Куб суммы:
	\begin{equation*}
	(a \pm b)^3 = (a^2 \pm 2ab + b^2)(a \pm b) = a^3 \pm 3a^2 b + 3ab^2 \pm b^3
	\end{equation*}
	
	\item Сумма кубов:
	\begin{equation*}
	a^3 \pm b^3 = a^3 \mp a^2 b + ab^2 \pm a^2 b - ab^2 \pm b^3 =
	a(a^2 \mp ab + b^2) \pm b(a^2 \mp ab + b^2) = (a \pm b)(a^2 \mp ab + b^2)
	\end{equation*}
\end{enumerate}

\begin{theorem}[формула бинома Ньютона]
\label{eq:binomial_expansion}
\begin{equation*}
\forall n \in \mathbb N \ (a + b)^n = \sum_{m=0}^n C_n^m a^{n-m} b^m
\end{equation*}
\end{theorem}
\begin{proofmathind}
	\indbase $n = 1$: $(a + b)^1 = a + b = C_1^0 a + C_1^1 b$
	\indstep Пусть формула верна для~$n$. Докажем истинность для~$n + 1$.
	\begin{equation*}
	(a + b)^{n+1} =
	(a + b)\sum_{m=0}^n C_n^m a^{n-m} b^m =
	\sum_{m=0}^n C_n^m a^{n-m+1} b^m + \sum_{m=0}^n C_n^m a^{n-m} b^{m+1} =
	\end{equation*}
	\begin{equation*}
	= a^{n+1} + \sum_{m=0}^{n-1} C_n^{m+1} a^{n-m} b^{m+1} + \sum_{m=0}^{n-1} C_n^m a^{n-m} b^{m+1} =
	a^{n+1} + \sum_{m=0}^{n-1} C_{n+1}^{m+1} a^{n-m} b^{m+1} + b^{n+1} =
	\end{equation*}
	\begin{equation*}
	= a^{n+1} + \sum_{m=1}^n C_{n+1}^m a^{n+1-m} b^m + b^{n+1} =
	\sum_{m=0}^{n+1} C_{n+1}^m a^{n+1-m} b^m
	\end{equation*} \indend
\end{proofmathind}