\subsection{Таблица первообразных}
\begin{itemize}
	\item $\displaystyle \int x^n\,dx = \frac{x^{n+1}}{n + 1} + C, \ n \neq -1$
	
	\item $\displaystyle \int \frac{dx}{x + a} = \ln |x + a| + C$
	\begin{proof}
	\begin{equation*}
	(\ln |x + a| + C)' = (\ln \sqrt{(x + a)^2})' = \frac1{|x + a|} \cdot \frac1{2\sqrt{(x + a)^2}} \cdot 2(x + a) = \frac1{x + a}
	\end{equation*}
	\end{proof}
	
	\item $\displaystyle \int \frac{dx}{x^2 + a^2} = \frac1a \arctg \frac{x}a + C, \ a \neq 0$
	\begin{proof}
	\begin{equation*}
	\int \frac{dx}{x^2 + a^2} =
	\frac1{a^2} \int \frac{dx}{1 + \left( \frac{x}a \right)^2} =
	\frac1a \int \frac{d \left( \frac{x}a \right)}{1 + \left( \frac{x}a \right)^2} =
	\frac1a \arctg \frac{x}a + C
	\end{equation*}
	\end{proof}
	
	\item $\displaystyle \int \frac{dx}{x^2 - a^2} = \frac1{2a} \ln \left| \frac{x - a}{x + a} \right| + C, \ a \neq 0$
	\begin{proof}
	\begin{equation*}
	\int \frac{dx}{x^2 - a^2} =
	\end{equation*}
	\end{proof}
	
	\item $\displaystyle \int \frac{x}{x^2 + a} dx = \frac12 \ln |x^2 + a| + C, \ a \neq 0$
	\begin{proof}
	\begin{equation*}
	\int \frac{x}{x^2 + a} dx =
	\frac12 \int \frac{d(x^2 + a)}{x^2 + a} =
	\frac12 \ln |x^2 + a| + C
	\end{equation*}
	\end{proof}
	
	\item $\displaystyle \int \frac{dx}{\sqrt{x^2 + a}} = \ln |x + \sqrt{x^2 + a}| + C, \ a \neq 0$
	\begin{proof}
	\begin{equation*}
	\int \frac{dx}{\sqrt{x^2 + a}} =
	\end{equation*}
	\end{proof}
	
	\item $\displaystyle \int \frac{dx}{\sqrt{a^2 - x^2}} = \arcsin \frac{x}a + C, \ a \neq 0$
	\begin{proof}
	\begin{equation*}
	\int \frac{dx}{\sqrt{a^2 - x^2}} =
	\end{equation*}
	\end{proof}
	
	\item $\displaystyle \int \frac{x}{\sqrt{a^2 \pm x^2}} dx = \pm \sqrt{a^2 \pm x^2} + C, \ a \neq 0$
	\begin{proof}
	\begin{equation*}
	\int \frac{x}{\sqrt{a^2 \pm x^2}} dx =
	\pm \frac12 \int (a^2 \pm x^2)^{-\tfrac12} d(a^2 \pm x^2) =
	\pm \sqrt{a^2 \pm x^2} + C
	\end{equation*}
	\end{proof}
	
	\item $\displaystyle \int a^x\,dx = \frac{a^x}{\ln a} + C$
	
	\item $\displaystyle \int \ln x\,dx = x \ln x - x + C$
	\begin{proof}
	\begin{equation*}
	\int \ln x\,dx =
	\int \ln x \cdot 1 \cdot dx =
	x \ln x - \int \frac{x}x dx =
	x \ln x - x + C
	\end{equation*}
	\end{proof}
	
	\item $\displaystyle \int \sin x\,dx = -\cos x + C$
	
	\item $\displaystyle \int \cos x\,dx = \sin x + C$
	
	\item $\displaystyle \int \frac{dx}{\cos^2 x} = \tg x + C$
	
	\item $\displaystyle \int \frac{dx}{\sin^2 x} = -\ctg x + C$
	
	\item $\displaystyle \int \tg x\,dx = -\ln |\cos x| + C$
	\begin{proof}
	\begin{equation*}
	\int \tg x\,dx =
	\int \frac{\sin x}{\cos x} dx =
	-\int \frac{d(\cos x)}{\cos x} =
	-\ln |\cos x| + C
	\end{equation*}
	\end{proof}
	
	\item $\displaystyle \int \ctg x\,dx = \ln |\sin x| + C$
	\begin{proof}
	\begin{equation*}
	\int \ctg x\,dx =
	\int \frac{\cos x}{\sin x} dx =
	\int \frac{d(\sin x)}{\sin x} =
	\ln |\sin x| + C
	\end{equation*}
	\end{proof}
	
	\item $\displaystyle \int \arcsin x\,dx = x \arcsin x + \sqrt{1 - x^2} + C$
	\begin{proof}
	\begin{equation*}
	\int \arcsin x =
	\int \arcsin x \cdot 1 \cdot dx =
	x \arcsin x - \int \frac{x}{\sqrt{1 - x^2}} dx =
	\end{equation*}
	\begin{equation*}
	= x \arcsin x + \frac12 \int (1 - x^2)^{-\tfrac12} d(1 - x^2) =
	x \arcsin x + \sqrt{1 - x^2} + C
	\end{equation*}
	\end{proof}
	
	\item $\displaystyle \int \arccos x\,dx = x \arccos x - \sqrt{1 - x^2} + C$
	\begin{proof}
	\begin{equation*}
	\int \arccos x =
	\int \arccos x \cdot 1 \cdot dx =
	x \arccos x + \int \frac{x}{\sqrt{1 - x^2}} dx =
	\end{equation*}
	\begin{equation*}
	= x \arccos x - \frac12 \int (1 - x^2)^{-\tfrac12} d(1 - x^2) =
	x \arccos x - \sqrt{1 - x^2} + C
	\end{equation*}
	\end{proof}
	
	\item $\displaystyle \int \arctg x\,dx = x \arctg x - \frac12 \ln |1 + x^2| + C$
	\begin{proof}
	\begin{equation*}
	\int \arctg x =
	\int \arctg x \cdot 1 \cdot dx =
	x \arctg x - \int \frac{x}{1 + x^2} dx =
	\end{equation*}
	\begin{equation*}
	= x \arctg x - \frac12 \int \frac{d(1 + x^2)}{1 + x^2} =
	x \arctg x - \frac12 \ln |1 + x^2| + C
	\end{equation*}
	\end{proof}
	
	\item $\displaystyle \int \arcctg x\,dx = x \arcctg x + \frac12 \ln |1 + x^2| + C$
	\begin{proof}
	\begin{equation*}
	\int \arcctg x =
	\int \arcctg x \cdot 1 \cdot dx =
	x \arcctg x + \int \frac{x}{1 + x^2} dx =
	\end{equation*}
	\begin{equation*}
	= x \arcctg x + \frac12 \int \frac{d(1 + x^2)}{1 + x^2} =
	x \arcctg x + \frac12 \ln |1 + x^2| + C
	\end{equation*}
	\end{proof}
\end{itemize}